formalization/thesis/Isotope/Forsp/Defs.lean
@@ -1,0 +1,89 @@
+import Isotope.SExp2.Defs
+
+namespace Isotope
+
+universe ua up
+
+namespace Forsp
+
+inductive Word (P : Type up) (A : Type ua) : Type _
+| prim (p : P)
+| atom (a : A)
+| push
+| pop
+| quote
+
+inductive SWord (P : Type up) (A : Type ua) : Type _
+| com (c : Word P A)
+| ref (a : A)
+| get (a : A)
+| set (a : A)
+
+variable {P A}
+
+instance Prim.instCoePrim : Coe P (Word P A) where
+  coe := .prim
+
+instance Word.instCoeAtom : Coe A (Word P A) where
+  coe := .atom
+
+instance SWord.instCoeWord : Coe (Word P A) (SWord P A) where
+  coe := .com
+
+def Prog (P : Type up) (A : Type ua) : Type _ := SExp2 (SWord P A)
+
+universe un uv us
+
+class StackM
+  (m : Type uv → Type us)
+  (Val : Type uv)
+  (State : Type uv)
+  where
+  pushM : Val → State → m State
+  popM : State → m (Val × State)
+
+structure PopEmptyStack where
+
+instance StackM.instList {m Val}
+  [Pure m] [MonadExcept PopEmptyStack m]
+  : StackM m Val (List Val) where
+  pushM v s := pure (v :: s)
+  popM
+    | [] => throw PopEmptyStack.mk
+    | v :: s => pure (v, s)
+
+class EnvM
+  (m : Type uv → Type us)
+  (Name : Type un) (Val : Type uv)
+  (State : Type uv)
+  where
+  getM : Name → State → m Val
+  setM : Name → Val → State → m State
+
+structure EnvNotFound (Name : Type _)
+
+class StoreM
+  (m : Type uv → Type us)
+  (Name : Type un) (Val : Type uv)
+  (State : Type uv)
+  extends
+  StackM m Val State,
+  EnvM m Name Val State
+
+structure Store (Stack : Type uv) (Env : Type uv) where
+  stack : Stack
+  env : Env
+
+-- instance StoreM.instStore
+--   {Val State Env Stack : Type uv}
+--   {Name : Type un}
+--   [StackM m Val State] [EnvM m Name Val Env]
+--   : StoreM m Name Val (Store Stack Env) where
+--   pushM := sorry
+--   popM := sorry
+--   getM := sorry
+--   setM := sorry
+
+end Forsp
+
+end Isotope
