formalization/thesis/Isotope/SExp2/Defs.lean
@@ -1,0 +1,58 @@
+import Mathlib.Data.List.OfFn
+
+namespace Isotope
+
+universe ua
+
+inductive SExp2 (A : Type ua) : Type ua where
+  | cons : SExp2 A → SExp2 A → SExp2 A
+  | nil : SExp2 A
+  | atom : A → SExp2 A
+
+namespace SExp2
+
+variable {A}
+
+@[simp]
+def fromList : List (SExp2 A) → SExp2 A
+  | .nil => .nil
+  | .cons a as => .cons a (fromList as)
+
+instance instCoeList : Coe (List (SExp2 A)) (SExp2 A) where
+  coe := fromList
+
+theorem coe_nil : (([] : List (SExp2 A)) : SExp2 A) = .nil := by simp
+
+theorem coe_cons (a : SExp2 A) (as : List (SExp2 A)) :
+  ((a :: as : List (SExp2 A)) : SExp2 A) = .cons a as
+  := by simp
+
+instance instEmptyCollection : EmptyCollection (SExp2 A) where
+  emptyCollection := .nil
+
+instance instInhabited : Inhabited (SExp2 A) where
+  default := .nil
+
+@[simp]
+def car : SExp2 A → Option (SExp2 A)
+  | .cons a _ => some a
+  | .nil => .some .nil
+  | .atom _ => none
+
+@[simp]
+def cdr : SExp2 A → Option (SExp2 A)
+  | .cons _ d => some d
+  | .nil => .some .nil
+  | .atom _ => none
+
+@[simp]
+def car' (e : SExp2 A) : SExp2 A
+  := e.car.getD .nil
+
+@[simp]
+def cdr' (e : SExp2 A) : SExp2 A
+  := e.cdr.getD .nil
+
+end SExp2
+
+end Isotope
