thesis/main.typ
@@ -3,8 +3,6 @@
 #show: thesis.with(
   title: "Categorical Imperative Programming",
   subtitle: "Type theory, refinement, and semantics for SSA",
-  author: "Jad-Elkhaleq Ghalayini",
-  date: datetime(day: 28, month: 3, year: 2026),
 )
 
 #include "intro/main.typ"
