thesis/type-theoretic-ssa/main.typ
@@ -1,5 +1,5 @@
 #import "/lib/prelude.typ": *
-#show: part
+#show: part.with(title: "Type-Theoretic SSA")
 
 The goal of this thesis is to study the formal semantics of SSA
 --
@@ -8,42 +8,7 @@ we will instead take a page from the "nanopass" school of compiler development
 and study various intermediate languages $L$,
 along with the _relationships_ between them.
 
-That means that the first few chapters of this thesis are going to be a bit repetitive: 
-for each language $L$ that we introduce, 
-after we've given some informal intuition and examples
-and situated it in our hierarchy of intermediate representations,
-we're going to need to give a formal description of the language 
-so that we can make precise and prove our claims.
-
-Usually, this means a variant of the following narrative:
-
-- We give $L$ a formal syntax
-  -- usually parametrized by abstract sets of operations and constants
-
-- We'll then often formalize $L$'s "expected" behaviour by 
-  equipping it with a simple _operational semantics_
-  --
-  typically, we will "build up" to a full semantics for $L$,
-  by starting with a simple rewriting-based semantics and then
-  adding features like _state_ and _nondeterminism_ in stages. 
-
-- Then, we define _type theory_ for $L$, consisting of:
-
-  - A _type system_
-    -- which defines the types a term can have 
-    and the contexts in which they are interpreted.
-    Usually, this will be parametrized by an abstract set of _base types_.
-
-    Often, we will study many different languages 
-    using the same type system.
-
-  - A _typing relation_
-    -- this typically consists of _typing rules_
-    which tell us which terms are well-typed in a given context.
-
-  - An _equational theory_ 
-    -- this gives us a notion of which terms may be considered _equivalent_
-    within a given context
+#todo[Fix segue]
 
 At this point, we've got a formal specification for a programming language:
 
@@ -64,9 +29,6 @@ At this point, we've got a formal specification for a programming language:
   we might be able to interpret $x + x$ as an integer in the context $x : ℤ$,
   or as a string in the context $x : #`str`$
   -- but $x + x$ doesn't make sense for $x : #`POBox`$.
-
-- An _operational semantics_ which describes an _abstract machine_
-  and tells us how to _execute_ our programs on it
 
 - An _equational theory_ which tells us when two terms are "the same" 
   in a particular context
@@ -106,20 +68,54 @@ Once we _have_ such a specification, however, the question remains as to whether
   -- how do we even _define_ two programs to be equivalent,
   in the presence of side-effects?
 
-#todo[
-  denotational semantics -- do we pull the operational semantics _down_? 
-  
-  do we even want it at all -- 
-  - it's not part of the MVP...
-  - but it really helps justify our denotational semantics as correct
-    -- otherwise completeness seems particularly abstract
-]
+#todo[Fix segue]
+
+
+That means that the first few chapters of this thesis are going to be a bit repetitive: 
+for each language $L$ that we introduce, 
+after we've given some informal intuition and examples
+and situated it in our hierarchy of intermediate representations,
+we're going to need to give a formal description of the language 
+so that we can make precise and prove our claims.
+
+Usually, this means a variant of the following narrative:
+
+- We give $L$ a formal syntax
+  -- usually parametrized by abstract sets of operations and constants
+
+/*
+
+TODO: opsem is a bonus, but is also about "grounding our programs in reality"
+
+- We'll then often formalize $L$'s "expected" behaviour by 
+  equipping it with a simple _operational semantics_
+  --
+  typically, we will "build up" to a full semantics for $L$,
+  by starting with a simple rewriting-based semantics and then
+  adding features like _state_ and _nondeterminism_ in stages. 
+*/
+
+- Then, we define _type theory_ for $L$, consisting of:
+
+  - A _type system_
+    -- which defines the types a term can have 
+    and the contexts in which they are interpreted.
+    Usually, this will be parametrized by an abstract set of _base types_.
+
+    Often, we will study many different languages 
+    using the same type system.
+
+  - A _typing relation_
+    -- this typically consists of _typing rules_
+    which tell us which terms are well-typed in a given context.
+
+  - An _equational theory_ 
+    -- this gives us a notion of which terms may be considered _equivalent_
+    within a given context
 
 #pagebreak()
 
 = S-Expressions
-
-#todo[This include should shift heading levels down by 1]
 
 #include "s-expressions/main.typ"
 
